scheduler/example/SCHMainA.v
@@ -12,10 +12,10 @@ Set Implicit Arguments.
 Module SCHMainA. Section SCHMainA.
   Context `{_crisG: !crisG Γ Σ α β τ _S _I, _concG: !concGS}.
   Context `{_schG: !SchA.schGS}.
-  Context `{_rrsG: !RRSA.rrsG}.
-  Context `{_ndsG: !NDSA.ndsG}.
+  Context `{_rrsG: !RRSA.rrsGS}.
+  Context `{_ndsG: !NDSA.ndsGS}.
   Context `{_memGS: !MemA.memGS}.
-  Context `{_nodeG: !RRSNodeA.nodeG}.
+  Context `{_nodeG: !RRSNodeA.nodeGS}.
   Import SCHMainI.
 
   Definition main_spec E : fspec :=
@@ -28,19 +28,17 @@ Module SCHMainA. Section SCHMainA.
     {[speckey_entry := fspec_to_rel (main_spec E)]}.
 
   Definition fnsems (E : coPset) : fnsemmap :=
-    {[None := Some (msk_scp ∅ msk_true, (fsp_some (main_spec E), main))]}.
+    {[None := Some (msk_scp [] msk_true, (fsp_some (main_spec E), main))]}.
 
   Program Definition smod E: SMod.t :=
     {|
-      SMod.scopes := ∅;
+      SMod.scopes := [];
       SMod.fnsems := fnsems E;
       SMod.initial_st := ∅;
     |}.
   Solve All Obligations with mod_tac.
 
-  Definition init_cond : iProp Σ :=
-    RRSAS.InitRRS ∗ RRSNodeAS.full_val (Vint 0) ∗ NDSA.InitNDS
-    ∗ own base_γ (gmap_view_frag 0 (DfracOwn 1) (to_agree 0)).
+  Definition init_cond : iProp Σ := RRSAS.InitRRS ∗ RRSNodeAS.full_val (Vint 0) ∗ NDSA.InitNDS.
 
   Definition t sp := SMod.to_mod sp (smod ⊤).
 End SCHMainA. End SCHMainA.
